\subsection{$\displaystyle \lim_{x\to \infty}\bracket[s]{\sqrt{x^2-x}-x}$}
\begin{gather}
\begin{aligned}
    \sqrt{x^2-x}-x &= \bracket{\sqrt{x^2-x}-x} \cdot \frac{\sqrt{x^2-x}+x}{\sqrt{x^2-x}+x}
    = \frac{\bracket{\sqrt{x^2-x}-x}\bracket{\sqrt{x^2-x}+x}}{\sqrt{x^2-x}+x}\\
    &= \frac{\bracket{\sqrt{x^2-x}}^2-x^2}{\sqrt{x^2-x}+x} 
    = \frac{x^2-x-x^2}{\sqrt{x^2-x}+x} = \frac{-x}{\sqrt{x^2-x}+x}\\
    &= \frac{-1}{\frac{1}{x}\sqrt{x^2-x}+1} = -\frac{1}{\sqrt{\frac{x^2}{x^2}-\frac{x}{x^2}}+1}
    = -\frac{1}{\sqrt{1-\frac{1}{x}}+1}  
\end{aligned}
\end{gather}
\begin{gather}
    \lim_{x\to\infty} \bracket[s]{\sqrt{x^2-x}-x} 
    = \lim_{x\to\infty} -\frac{1}{\sqrt{1-\frac{1}{x}}+1} \\
    \mbox{as } x \to \infty\mbox{: } \frac{1}{x} \to  0^+; \quad \sqrt{1-\frac{1}{x}} \to  1^-;
    \quad \sqrt{1-\frac{1}{x}}+1 \to 2^-\\
    \result{\lim_{x\to\infty} \bracket[s]{\sqrt{x^2-x}-x} = -\frac{1}{2}^-= -0.5^-}
\end{gather}
